Update Imp.v

Imp.v
@@ -28,3 +28,257 @@ Proof.
   try (rewrite optimize_0plus_sound);
   reflexivity.
 Qed.
+
+(** Exercise: (bevalR) **)
+(* Write a relation [bevalR] in the same style as
+    [aevalR], and prove that it is equivalent to [beval].*)
+    
+Reserved Notation "e '//' n" (at level 50, left associativity).
+
+Inductive bevalR: bexp -> bool -> Prop :=
+  | E_BTrue : BTrue // true
+  | E_BFalse : BFalse // false
+  | E_BEq : forall (e1 e2: aexp) (n1 n2 : nat),
+    e1 \\ n1 ->
+    e2 \\ n2 ->
+    BEq e1 e2 // (beq_nat n1 n2)
+  | E_BLe : forall (e1 e2: aexp) (n1 n2 : nat),
+    e1 \\ n1 ->
+    e2 \\ n2 ->
+    BLe e1 e2 // (ble_nat n1 n2)
+  | E_BNot : forall (e: bexp) (b:bool), 
+    BNot e // negb b
+  | E_BAnd : forall (e1 e2: bexp) (b1 b2: bool), 
+    BAnd e1 e2 // b1 && b2
+
+   where "e '//' n" := (bevalR e n) : type_scope.
+
+Reserved Notation "e '\\' n" (at level 50, left associativity).
+
+(** **** Exercise: (ceval_example2)  *)
+Example ceval_example2:
+    (X ::= ANum 0;; Y ::= ANum 1;; Z ::= ANum 2) / empty_state \\
+    (t_update (t_update (t_update empty_state X 0) Y 1) Z 2).
+Proof.
+  apply E_Seq with (t_update empty_state X 0).
+  - apply E_Ass. reflexivity.
+  - apply E_Seq with (t_update (t_update empty_state X 0) Y 1);
+    (apply E_Ass; reflexivity).
+Qed.
+
+
+(** **** Exercise: (pup_to_n)  *)
+(** Write an Imp program that sums the numbers from [1] to
+   [X] (inclusive: [1 + 2 + ... + X]) in the variable [Y].
+   Prove that this program executes as intended for [X] = [2]
+   (the latter is trickier than you might expect). *)
+
+Definition pup_to_n : com :=
+  Y ::= ANum 0 ;;
+  WHILE BNot (BEq (AId X) (ANum 0)) DO
+  Y ::= APlus (AId Y) (AId X) ;;
+  X ::= AMinus (AId X) (ANum 1)
+  END.
+
+Theorem pup_to_2_ceval :
+  pup_to_n / (t_update empty_state X 2) \\
+    t_update (t_update (t_update (t_update (t_update (t_update empty_state
+      X 2) Y 0) Y 2) X 1) Y 3) X 0.
+Proof.
+  apply E_Seq with (t_update (t_update empty_state X 2) Y 0) .
+  - apply E_Ass. reflexivity.
+  - apply E_WhileLoop with (t_update (t_update (t_update (t_update empty_state X 2) Y 0) Y 2) X 1).
+    + reflexivity.
+    + apply E_Seq with (t_update (t_update (t_update empty_state X 2) Y 0) Y 2);
+      (apply E_Ass; reflexivity).
+    + apply E_WhileLoop with (t_update (t_update (t_update (t_update (t_update (t_update empty_state X 2) Y 0) Y 2) X 1) Y 3) X 0).
+      * reflexivity.
+      * apply E_Seq with (t_update (t_update (t_update (t_update (t_update empty_state X 2) Y 0) Y 2) X 1) Y 3);
+        (apply E_Ass; reflexivity).
+      * apply E_WhileEnd. reflexivity.
+Qed.
+
+(** **** Exercise: (loop_never_stops)  *)
+Theorem loop_never_stops : forall st st',
+  ~(loop / st \\ st').
+Proof.
+  intros st st' contra. unfold loop in contra.
+  remember (WHILE BTrue DO SKIP END) as loopdef
+           eqn:Heqloopdef.
+
+  (** Proceed by induction on the assumed derivation showing that
+      [loopdef] terminates.  Most of the cases are immediately
+     contradictory (and so can be solved in one step with inversion).*)
+  induction contra; inversion Heqloopdef; subst.
+  simpl in H. inversion H. 
+  apply IHcontra2. reflexivity.
+Qed.
+
+(** **** Exercise: (no_whilesR)  *)
+(** Consider the definition of the [no_whiles] boolean predicate below: *)
+
+Fixpoint no_whiles (c : com) : bool :=
+  match c with
+  | SKIP =>
+      true
+  | _ ::= _ =>
+      true
+  | c1 ;; c2 =>
+      andb (no_whiles c1) (no_whiles c2)
+  | IFB _ THEN ct ELSE cf FI =>
+      andb (no_whiles ct) (no_whiles cf)
+  | WHILE _ DO _ END  =>
+      false
+  end.
+
+(** This predicate yields [true] just on programs that have no while
+    loops.  Using [Inductive], write a property [no_whilesR] such that
+    [no_whilesR c] is provable exactly when [c] is a program with no
+    while loops.  Then prove its equivalence with [no_whiles]. *)
+
+Inductive no_whilesR: com -> Prop :=
+| nowhile_skip : no_whilesR SKIP
+| nowhile_ass : forall id val, 
+    no_whilesR (id ::= val)
+| nowhile_seq : forall c1 c2, 
+    no_whilesR c1 ->
+    no_whilesR c2 ->
+    no_whilesR (c1 ;; c2)
+| nowhile_if : forall b ct cf, 
+    no_whilesR ct ->
+    no_whilesR cf ->
+    no_whilesR (IFB b THEN ct ELSE cf FI).
+
+Theorem no_whiles_eqv:
+   forall c, no_whiles c = true <-> no_whilesR c.
+Proof.
+  split.
+  - intros H. induction c; simpl in H;
+          try(apply andb_true_iff in H; destruct H);
+          try(constructor);
+          try (apply IHc1);
+          try (apply IHc2); try(assumption).
+          inversion H.
+  - intros. induction H; try (reflexivity);
+    simpl; rewrite IHno_whilesR1; rewrite IHno_whilesR2;
+    reflexivity.
+Qed.
+
+(* ################################################################# *)
+(** * Additional Exercises *)
+
+(** **** Exercise: (stack_compiler)  *)
+(** HP Calculators, programming languages like Forth and Postscript,
+    and abstract machines like the Java Virtual Machine all evaluate
+    arithmetic expressions using a stack. For instance, the expression
+
+      (2*3)+(3*(4-2))
+
+   would be entered as
+
+      2 3 * 3 4 2 - * +
+
+   and evaluated like this (where we show the program being evaluated 
+   on the right and the contents of the stack on the left):
+
+      []            |    2 3 * 3 4 2 - * +
+      [2]           |    3 * 3 4 2 - * +
+      [3, 2]        |    * 3 4 2 - * +
+      [6]           |    3 4 2 - * +
+      [3, 6]        |    4 2 - * +
+      [4, 3, 6]     |    2 - * +
+      [2, 4, 3, 6]  |    - * +
+      [2, 3, 6]     |    * +
+      [6, 6]        |    +
+      [12]          |
+
+  The task of this exercise is to write a small compiler that
+  translates [aexp]s into stack machine instructions.
+
+  The instruction set for our stack language will consist of the
+  following instructions:
+     - [SPush n]: Push the number [n] on the stack.
+     - [SLoad x]: Load the identifier [x] from the store and push it
+                  on the stack
+     - [SPlus]:   Pop the two top numbers from the stack, add them, and
+                  push the result onto the stack.
+     - [SMinus]:  Similar, but subtract.
+     - [SMult]:   Similar, but multiply. *)
+
+Inductive sinstr : Type :=
+| SPush : nat -> sinstr
+| SLoad : id -> sinstr
+| SPlus : sinstr
+| SMinus : sinstr
+| SMult : sinstr.
+
+(** Write a function to evaluate programs in the stack language. It
+    should take as input a state, a stack represented as a list of
+    numbers (top stack item is the head of the list), and a program
+    represented as a list of instructions, and it should return the
+    stack after executing the program.  Test your function on the
+    examples below.
+
+    Note that the specification leaves unspecified what to do when
+    encountering an [SPlus], [SMinus], or [SMult] instruction if the
+    stack contains less than two elements.  In a sense, it is
+    immaterial what we do, since our compiler will never emit such a
+    malformed program. *)
+
+Fixpoint s_execute (st : state) (stack : list nat)
+                   (prog : list sinstr)
+                 : list nat :=
+ match prog with
+   | [] => stack
+   | first_c :: commands => match first_c with
+                           | SPush n => s_execute st (n :: stack) commands (* lo añadimos a la lista pila *)
+                           | SLoad i => s_execute st (st i :: stack) commands
+                           | SPlus => match stack with
+                                       | f :: s :: t => s_execute st ((f+s) :: t) commands
+                                       | _ => s_execute st stack commands
+                                      end
+                           | SMinus => match stack with
+                                        | f :: s :: t => s_execute st ((s - f) :: t) commands
+                                        | _ => s_execute st stack commands
+                                       end
+                           | SMult => match stack with
+                                       | f :: s :: t => s_execute st ((s * f) :: t) commands
+                                       | _ => s_execute st stack commands
+                                      end
+                           end
+  end.
+
+
+Example s_execute1 :
+     s_execute empty_state []
+       [SPush 5; SPush 3; SPush 1; SMinus]
+   = [2; 5].
+Proof. reflexivity. Qed.
+
+Example s_execute2 :
+     s_execute (t_update empty_state X 3) [3;4]
+       [SPush 4; SLoad X; SMult; SPlus]
+   = [15; 4].
+Proof. reflexivity. Qed.
+
+(** Next, write a function that compiles an [aexp] into a stack
+    machine program. The effect of running the program should be the
+    same as pushing the value of the expression on the stack. *)
+
+Fixpoint s_compile (e : aexp) : list sinstr :=
+  match e with
+    | ANum n1 => [SPush n1]
+    | AId i => [SLoad i]
+    | APlus e1 e2 => (s_compile e1) ++ (s_compile e2) ++ [SPlus]
+    | AMinus e1 e2 => (s_compile e1) ++ (s_compile e2) ++ [SMinus]
+    | AMult e1 e2 => (s_compile e1) ++ (s_compile e2) ++ [SMult]
+
+  end.
+
+(** After you've defined [s_compile], prove the following to test
+    that it works. *)
+
+Example s_compile1 :
+    s_compile (AMinus (AId X) (AMult (ANum 2) (AId Y)))
+  = [SLoad X; SPush 2; SLoad Y; SMult; SMinus].
+Proof. reflexivity. Qed.
